<?xml version="1.0"?>
<rdf:RDF xmlns="http://w3id.org/infocomm#"
     xml:base="http://w3id.org/infocomm"
     xmlns:owl="http://www.w3.org/2002/07/owl#"
     xmlns:rdf="http://www.w3.org/1999/02/22-rdf-syntax-ns#"
     xmlns:rdfs="http://www.w3.org/2000/01/rdf-schema#"
	 xmlns:terms="http://purl.org/dc/terms/">

    <owl:Ontology rdf:about="http://w3id.org/infocomm">
		<terms:title xml:lang="en">Information Communication Ontology</terms:title>
        <terms:description xml:lang="en">An ontology for describing information communication.</terms:description>
    </owl:Ontology>

    <!-- Classes with Definitions -->
	<owl:Class rdf:ID="CommunicationEvent">
        <rdfs:comment>The transport of information through space and/or time.</rdfs:comment>
    </owl:Class>
	
    <owl:Class rdf:ID="Information">
        <rdfs:comment>That which is communicated.</rdfs:comment>
		<rdfs:comment>Examples include, but are not limited to, ideas, knowledge, facts, claims, feelings and plans.</rdfs:comment>
    </owl:Class>

    <owl:Class rdf:ID="CommunicationParty">
        <rdfs:comment>An entity that participates in a communication event.</rdfs:comment>
    </owl:Class>

    <owl:Class rdf:ID="Medium">
        <rdfs:comment>A thing that is altered, either temporarily or permanently, to preserve information during a communication event.</rdfs:comment>
		<rdfs:comment>Radio waves (in wireless communication) and coaxial cables (in wired communication) are good examples.</rdfs:comment>
    </owl:Class>
	
	<owl:Class rdf:ID="Format">
        <rdfs:comment>The way in which a thing is altered to act as a medium during a communication event.</rdfs:comment>
		<rdfs:comment>Formats include things like JSON, CSV and PDF, but also things like UTF-8 or base64 encoding.</rdfs:comment>
		<rdfs:comment>An encoding system (in computer terms) is an example of a format.</rdfs:comment>
    </owl:Class>

    <owl:Class rdf:ID="Protocol">
        <rdfs:comment>A set of rules governing a communication event.</rdfs:comment>
		<rdfs:comment>Bluetooth, SMS, TCP/IP are all examples of communication protocols.</rdfs:comment>
		<rdfs:comment>A language (e.g., English or Spanish) may be regarded as a protocol in itself.</rdfs:comment>
    </owl:Class>

    <!-- Object Properties -->
    <owl:ObjectProperty rdf:ID="hasSender">
        <rdfs:domain rdf:resource="#CommunicationEvent"/>
        <rdfs:range rdf:resource="#CommunicationParty"/>
		<owl:inverseOf rdf:resource="#senderOf"/>
		<rdfs:comment>A communication party fulfils the 'sender' role if they transmit the communicated information.</rdfs:comment>
    </owl:ObjectProperty>

    <owl:ObjectProperty rdf:ID="hasRecipient">
        <rdfs:domain rdf:resource="#CommunicationEvent"/>
        <rdfs:range rdf:resource="#CommunicationParty"/>
		<owl:inverseOf rdf:resource="#recipientOf"/>
		<rdfs:comment>A communication party fulfils the 'recipient' role if they receive the communicated information.</rdfs:comment>
    </owl:ObjectProperty>

    <owl:ObjectProperty rdf:ID="hasMedium">
        <rdfs:domain rdf:resource="#CommunicationEvent"/>
        <rdfs:range rdf:resource="#Medium"/>
        <!-- <rdf:type rdf:resource="http://www.w3.org/2002/07/owl#FunctionalProperty"/> -->
    </owl:ObjectProperty>

	<owl:ObjectProperty rdf:ID="hasFormat">
        <rdfs:domain rdf:resource="#CommunicationEvent"/>
        <rdfs:range rdf:resource="#Format"/>
        <!-- <rdf:type rdf:resource="http://www.w3.org/2002/07/owl#FunctionalProperty"/> -->
    </owl:ObjectProperty>

	<owl:ObjectProperty rdf:ID="governs">
        <rdfs:domain rdf:resource="#Protocol"/>
        <rdfs:range rdf:resource="#CommunicationEvent"/>
		<owl:inverseOf rdf:resource="#isGovernedBy"/>
    </owl:ObjectProperty>

    <owl:ObjectProperty rdf:ID="transmits">
        <rdfs:domain rdf:resource="#CommunicationEvent"/>
        <rdfs:range rdf:resource="#Information"/>
        <!-- <rdf:type rdf:resource="http://www.w3.org/2002/07/owl#FunctionalProperty"/> -->
    </owl:ObjectProperty>
	

    <!-- Disjoint Classes -->
    <owl:AllDisjointClasses>
        <owl:members rdf:parseType="Collection">
		    <rdf:Description rdf:about="#CommunicationEvent"/>
		    <rdf:Description rdf:about="#Information"/>
            <rdf:Description rdf:about="#CommunicationParty"/>
            <rdf:Description rdf:about="#Medium"/>
		    <rdf:Description rdf:about="#Format"/>
            <rdf:Description rdf:about="#Protocol"/>
        </owl:members>
    </owl:AllDisjointClasses>

</rdf:RDF>
