@prefix : <http://w3id.org/infocomm#> .
@prefix dcterms: <http://purl.org/dc/terms/> .
@prefix owl: <http://www.w3.org/2002/07/owl#> .
@prefix rdf: <http://www.w3.org/1999/02/22-rdf-syntax-ns#> .
@prefix rdfs: <http://www.w3.org/2000/01/rdf-schema#> .
@prefix skos: <http://www.w3.org/2004/02/skos/core#> .

<http://w3id.org/infocomm> a owl:Ontology ;
    dcterms:description "An ontology for describing information communication."@en ;
    dcterms:title "Information Communication Ontology"@en .

:governs a owl:ObjectProperty ;
    rdfs:label "governs"@en ;
    rdfs:domain :Protocol ;
    rdfs:range :CommunicationEvent ;
    owl:inverseOf :isGovernedBy .

:hasFormat a owl:ObjectProperty ;
    rdfs:label "hasFormat"@en ;
    rdfs:domain :CommunicationEvent ;
    rdfs:range :Format .

:hasMedium a owl:ObjectProperty ;
    rdfs:label "hasMedium"@en ;
    rdfs:domain :CommunicationEvent ;
    rdfs:range :Medium .

:hasRecipient a owl:ObjectProperty ;
    rdfs:label "hasRecipient"@en ;
    rdfs:comment "A communication party fulfils the 'recipient' role if they receive the communicated information." ;
    rdfs:domain :CommunicationEvent ;
    rdfs:range :CommunicationParty .

:hasSender a owl:ObjectProperty ;
    rdfs:label "hasSender"@en ;
    rdfs:comment "A communication party fulfils the 'sender' role if they transmit the communicated information." ;
    rdfs:domain :CommunicationEvent ;
    rdfs:range :CommunicationParty .

:recipientOf a owl:ObjectProperty ;
    rdfs:label "recipientOf"@en ;
    rdfs:domain :CommunicationParty ;
    rdfs:range :Information .

:senderOf a owl:ObjectProperty ;
    rdfs:label "senderOf"@en ;
    rdfs:domain :CommunicationParty ;
    rdfs:range :Information .

:transmits a owl:ObjectProperty ;
    rdfs:label "transmits"@en ;
    rdfs:domain :CommunicationEvent ;
    rdfs:range :Information .

:Format a owl:Class ;
    rdfs:label "Format"@en ;
    rdfs:comment "An encoding system (in computer terms) is an example of a format.",
        "Formats include things like JSON, CSV and PDF, but also things like UTF-8 or base64 encoding." ;
    skos:definition "The way in which a thing is altered to act as a medium during a communication event." .

:Medium a owl:Class ;
    rdfs:label "Medium"@en ;
    rdfs:comment "Radio waves (in wireless communication) and coaxial cables (in wired communication) are good examples." ;
    skos:definition "A thing that is altered, either temporarily or permanently, to preserve information during a communication event." .

:Protocol a owl:Class ;
    rdfs:label "Protocol"@en ;
    rdfs:comment "A language (e.g., English or Spanish) may be regarded as a protocol in itself.",
        "Bluetooth, SMS, TCP/IP are all examples of communication protocols." ;
    skos:definition "A set of rules governing a communication event." .

:Information a owl:Class ;
    rdfs:label "Information"@en ;
    rdfs:comment "Examples include, but are not limited to, ideas, knowledge, facts, claims, feelings and plans." ;
    skos:definition "That which is communicated." .

:CommunicationParty a owl:Class ;
    rdfs:label "CommunicationParty"@en ;
    skos:definition "An entity that participates in a communication event." .

:CommunicationEvent a owl:Class ;
    rdfs:label "CommunicationEvent"@en ;
    skos:definition "The transport of information through space and/or time." .

[] a owl:AllDisjointClasses ;
    owl:members ( :CommunicationEvent :Information :CommunicationParty :Medium :Format :Protocol ) .

